eve/Src/framework/eiffel2boogie/iv/iv_map_update.e
@@ -1,15 +1,12 @@
 note
-	description: "[
-		TODO
-	]"
+	description: "Map update expression."
 	date: "$Date$"
 	revision: "$Revision$"
 
 class
-	IV_MAP_ACCESS
+	IV_MAP_UPDATE
 
 inherit
-
 	IV_EXPRESSION
 
 	IV_SHARED_TYPES
@@ -19,18 +16,21 @@ create
 
 feature {NONE} -- Implementation
 
-	make (a_target: IV_EXPRESSION; a_indexes: ARRAY [IV_EXPRESSION])
-			-- Make map access to `a_target' with index `a_indexes'.
+	make (a_target: IV_EXPRESSION; a_indexes: ARRAY [IV_EXPRESSION]; a_value: IV_EXPRESSION)
+			-- Make map update of `a_target' at index `a_indexes' with `a_value'.
 		require
 			a_target_attached: attached a_target
 			a_target_valid: attached {IV_MAP_TYPE} a_target.type as t and then t.domain_types.count = a_indexes.count
 			a_indexes_attached: attached a_indexes and then across a_indexes as i all attached i.item end
+			a_value_attached: attached a_value
 		do
 			target := a_target
 			indexes := a_indexes
+			value := a_value
 		ensure
 			target_set: target = a_target
 			indexes_set: indexes = a_indexes
+			value_set: value = a_value
 		end
 
 feature -- Access
@@ -41,32 +41,27 @@ feature -- Access
 	indexes: ARRAY [IV_EXPRESSION]
 			-- Indexes.
 
+	value: IV_EXPRESSION
+			-- New value.
+
 	type: IV_TYPE
 			-- Type of map access.
 		do
-			check attached {IV_MAP_TYPE} target.type as map_type then
-				-- ToDo: find most general unifier of domain types with index types and instantiate the range type
-				-- For now a workaround: heap is the only map type with a polymorphic result we use
-				if map_type ~ types.heap then
-					check attached {IV_USER_TYPE} indexes [2].type as field_type then
-						Result := field_type.parameters [1]
-					end
-				else
-					Result := map_type.range_type
-				end
-			end
+			Result := target.type
 		end
 
 	triggers_for (a_bound_var: IV_ENTITY): ARRAYED_LIST [IV_EXPRESSION]
 			-- List of smallest subexpressions of `Current' with a valid triggers for a bound variable `a_bound_var'.			
 		do
 			create Result.make (3)
-			if across indexes as i some i.item.has_free_var_named (a_bound_var.name) and i.item.triggers_for (a_bound_var).is_empty end then
+			if across indexes as i some i.item.has_free_var_named (a_bound_var.name) and i.item.triggers_for (a_bound_var).is_empty end
+				or value.has_free_var_named (a_bound_var.name) and value.triggers_for (a_bound_var).is_empty then
 				Result.extend (Current)
 			else
 				across indexes as i loop
 					Result.append (i.item.triggers_for (a_bound_var))
 				end
+				Result.append (value.triggers_for (a_bound_var))
 			end
 		end
 
@@ -76,7 +71,8 @@ feature -- Status report
 			-- Does this expression contain a free variable with name `a_name'?
 		do
 			Result := target.has_free_var_named (a_name) or
-				across indexes as i some i.item.has_free_var_named (a_name) end
+				across indexes as i some i.item.has_free_var_named (a_name) end or
+				value.has_free_var_named (a_name)
 		end
 
 feature -- Comparison
@@ -84,10 +80,11 @@ feature -- Comparison
 	same_expression (a_other: IV_EXPRESSION): BOOLEAN
 			-- Does this expression equal `a_other' (if considered in the same context)?
 		do
-			Result := attached {IV_MAP_ACCESS} a_other as m and then
+			Result := attached {IV_MAP_UPDATE} a_other as m and then
 				(target.same_expression (m.target) and
 				indexes.count = m.indexes.count and
-				across 1 |..| indexes.count as i all indexes [i.item].same_expression (m.indexes [i.item]) end)
+				across 1 |..| indexes.count as i all indexes [i.item].same_expression (m.indexes [i.item]) end and
+				value.same_expression (m.value))
 		end
 
 feature -- Visitor
@@ -95,7 +92,7 @@ feature -- Visitor
 	process (a_visitor: IV_EXPRESSION_VISITOR)
 			-- <Precursor>
 		do
-			a_visitor.process_map_access (Current)
+			a_visitor.process_map_update (Current)
 		end
 
 invariant
@@ -103,5 +100,6 @@ invariant
 	indexes_attached: attached indexes
 	target_valid: attached {IV_MAP_TYPE} target.type as t and then t.domain_types.count = indexes.count
 	indexes_nonempty: not indexes.is_empty
+	value_attached: attached value
 
 end
