eve/Src/framework/eiffel2boogie/tests/framing/ownership/master_clock/f_mc_clock_d.e
@@ -2,7 +2,7 @@ note
 	description: "Slave clock whose time must not exceed its master's."
 	explicit: "all"
 
-frozen class F_MC_CLOCK_D
+class F_MC_CLOCK_D
 
 create
 	make
