eve/Src/framework/eiffel2boogie/tests/framing/ownership/master_clock/f_mc_master.e
@@ -22,6 +22,10 @@ feature -- Access
 
 	time: INTEGER
 			-- Time.
+		note
+			guard: time_increased
+		attribute
+		end
 
 feature -- Update			
 
@@ -30,7 +34,7 @@ feature -- Update
 		require
 			modify_field (["time", "closed"], Current)
 		do
-			-- This update preserves the invariant of slave clocks:
+			-- This update satisfies its guard and thus preserves the invariant of slave clocks:
 			time := time + 1
 		ensure
 			time_increased: time > old time
@@ -45,17 +49,26 @@ feature -- Update
 			observers_open: across observers as o all o.item.is_open end
 			modify_field (["time", "closed"], Current)
 		do
-			-- This update does not preserve the invariant of slave clocks,
-			-- so the method requires that they be open:
+			-- This update does not satisfy its guard,
+			-- so the method requires that the observers be open:
 			time := 0
 		ensure
 			wrapped: is_wrapped
 			time_reset: time = 0
 		end
 
+feature -- Specification
+
+	time_increased (new_time: INTEGER; o: ANY): BOOLEAN
+			-- Is `new_time' greater than `time'?
+		note
+			status: functional
+		do
+			Result := new_time >= time
+		end
+
 invariant
 	time_non_negative: 0 <= time
-	all_observers_are_clocks: across observers as o all attached {F_MC_CLOCK} o.item end
 
 note
 	explicit: observers
