eve/Src/framework/eiffel2boogie/tests/framing/ownership/master_clock/f_mc_master_d.e
@@ -27,6 +27,10 @@ feature -- Access
 
 	time: INTEGER
 			-- Time.
+		note
+			guard: time_increased
+		attribute
+		end
 
 feature -- Update			
 
@@ -38,7 +42,7 @@ feature -- Update
 			modify_field (["time", "closed"], Current)
 		do
 			unwrap
-			-- This update preserves the invariant of slave clocks:
+			-- This update satisfies its guard and thus preserves the invariant of slave clocks:
 			time := time + 1
 			wrap
 		ensure
@@ -54,8 +58,8 @@ feature -- Update
 			modify_field (["time", "closed"], Current)
 		do
 			unwrap
-			-- This update does not preserve the invariant of slave clocks,
-			-- so the method requires that they be open:
+			-- This update does not satisfy its guard,
+			-- so the method requires that the observers be open:
 			time := 0
 			wrap
 		ensure
@@ -63,9 +67,18 @@ feature -- Update
 			time_reset: time = 0
 		end
 
+feature -- Specification
+
+	time_increased (new_time: INTEGER; o: ANY): BOOLEAN
+			-- Is `new_time' greater than `time'?
+		note
+			status: functional
+		do
+			Result := new_time >= time
+		end
+
 invariant
 	time_non_negative: 0 <= time
-	all_observers_are_clocks: across observers as o all attached {F_MC_CLOCK_D} o.item end
 	default_owns: owns = []
 	default_subjects: subjects = []
 
