eve/Src/framework/eiffel2boogie/translation/across/e2b_across_handler.e
@@ -137,7 +137,7 @@ feature {NONE} -- Implementation
 			else
 				create {IV_EXISTS} Result.make (factory.and_ (l_guard, a_expr))
 			end
-			Result.add_bound_variable (a_bound_var.name, a_bound_var.type)
+			Result.add_bound_variable (a_bound_var)
 			if expression_translator.use_triggers then
 				add_triggers (Result)
 			end
